Thinking about splits...

Refinery/Ctx/Add.lean
@@ -4,6 +4,43 @@ namespace Refinery
 
 def Var?.add (v w : Var? α ε) : Var? α ε := ⟨v.ty, v.q + w.q, v.eff⟩
 
+structure Var?.compat (v w : Var? α ε) : Prop where
+  ty : v.ty = w.ty
+  eff : v.eff = w.eff
+
+@[simp]
+theorem Var?.compat.refl (v : Var? α ε) : Var?.compat v v := ⟨rfl, rfl⟩
+
+theorem Var?.compat.symm {v w : Var? α ε} (h : Var?.compat v w) : Var?.compat w v
+  := ⟨h.ty.symm, h.eff.symm⟩
+
+theorem Var?.compat.trans {u v w : Var? α ε} (huv : Var?.compat u v) (hvw : Var?.compat v w)
+  : Var?.compat u w := ⟨huv.ty.trans hvw.ty, huv.eff.trans hvw.eff⟩
+
+theorem Var?.compat.erase_left {v w : Var? α ε} (h : Var?.compat v w) : Var?.compat v.erase w
+  := ⟨h.ty, h.eff⟩
+
+theorem Var?.compat.erase_rigth {v w : Var? α ε} (h : Var?.compat v w) : Var?.compat v w.erase
+  := ⟨h.ty, h.eff⟩
+
+@[simp]
+theorem Var?.compat.self_erase_left (v : Var? α ε) : Var?.compat v.erase v := ⟨rfl, rfl⟩
+
+@[simp]
+theorem Var?.compat.self_erase_right (v : Var? α ε) : Var?.compat v v.erase := ⟨rfl, rfl⟩
+
+structure Var?.qcompat (v w : Var? α ε) extends compat v w : Prop where
+  q : v.q = w.q ∨ (v.q = 0 ∨ w.q = 0)
+
+@[simp]
+theorem Var?.qcompat.refl (v : Var? α ε) : Var?.qcompat v v := ⟨Var?.compat.refl v, Or.inl rfl⟩
+
+theorem Var?.qcompat.symm {v w : Var? α ε} (h : Var?.qcompat v w) : Var?.qcompat w v
+  := ⟨Var?.compat.symm h.tocompat, match h.q with
+    | Or.inl h => Or.inl h.symm
+    | Or.inr (Or.inl h) => Or.inr (Or.inr h)
+    | Or.inr (Or.inr h) => Or.inr (Or.inl h)⟩
+
 instance Var?.instAdd : Add (Var? α ε) where
   add := Var?.add
 
@@ -22,6 +59,36 @@ def Ctx?.add (Γ Δ : Ctx? α ε) : Ctx? α ε := match Γ, Δ with
   | .nil, Δ => Δ
   | Γ, .nil => Γ
   | .cons Γ v, .cons Δ w => .cons (Γ.add Δ) (v + w)
+
+inductive Ctx?.compat : Ctx? α ε → Ctx? α ε → Prop where
+  | nil : Ctx?.compat .nil .nil
+  | cons {Γ Δ} {v w : Var? α ε} (hΓ : Ctx?.compat Γ Δ) (hv : Var?.compat v w)
+    : Ctx?.compat (Γ.cons v) (Δ.cons w)
+
+@[simp]
+theorem Ctx?.compat.refl (Γ : Ctx? α ε) : Ctx?.compat Γ Γ := by
+  induction Γ <;> constructor <;> simp [*]
+
+theorem Ctx?.compat.symm {Γ Δ : Ctx? α ε} (h : Ctx?.compat Γ Δ) : Ctx?.compat Δ Γ := by
+  induction h <;> constructor <;> simp [Var?.compat.symm, *]
+
+theorem Ctx?.compat.trans {Γ Δ Ξ : Ctx? α ε} (hΓΔ : Ctx?.compat Γ Δ) (hΔΞ : Ctx?.compat Δ Ξ)
+  : Ctx?.compat Γ Ξ := by
+  induction hΓΔ generalizing Ξ <;> cases hΔΞ
+  <;> constructor; apply_assumption; assumption; apply Var?.compat.trans <;> assumption
+
+inductive Ctx?.qcompat : Ctx? α ε → Ctx? α ε → Prop where
+  | nil : Ctx?.qcompat .nil .nil
+  | cons {Γ Δ} {v w : Var? α ε} (hΓ : Ctx?.qcompat Γ Δ) (hv : Var?.qcompat v w)
+    : Ctx?.qcompat (Γ.cons v) (Δ.cons w)
+
+@[simp]
+theorem Ctx?.qcompat.refl (Γ : Ctx? α ε) : Ctx?.qcompat Γ Γ := by
+  induction Γ <;> constructor <;> simp [*]
+
+@[simp]
+theorem Ctx?.qcompat.symm (Γ Δ : Ctx? α ε) (h : Ctx?.qcompat Γ Δ) : Ctx?.qcompat Δ Γ := by
+  induction h <;> constructor <;> simp [Var?.qcompat.symm, *]
 
 instance Ctx?.instAdd : Add (Ctx? α ε) where
   add := Ctx?.add
@@ -47,3 +114,41 @@ instance AddMonoid : AddMonoid (Ctx? α ε) where
   zero_add Γ := Γ.nil_add
   add_zero Γ := Γ.add_nil
   nsmul := nsmulRec
+
+variable [HasQuant α]
+
+open HasQuant
+
+@[simp]
+theorem Var?.PSSplit.trg_compat {u v w : Var? α ε} (h : u.PSSplit v w) : v.compat w := by
+  cases h <;> simp
+
+@[simp]
+theorem Var?.PSSplit.left_compat {u v w : Var? α ε} (h : u.PSSplit v w) : u.compat v := by
+  cases h <;> simp
+
+@[simp]
+theorem Var?.PSSplit.right_compat {u v w : Var? α ε} (h : u.PSSplit v w) : u.compat w := by
+  cases h <;> simp
+
+@[simp]
+theorem Var?.add_idem_copy (v : Var? α ε) [hv : v.copy] : v + v = v := by
+  cases v with | mk A q e =>
+  simp only [add_def, mk.injEq, and_true, true_and]
+  cases q using EQuant.casesZero with
+  | zero => rfl
+  | rest q =>
+    simp [copy_iff] at hv
+    cases hv.q using EQuant.le.casesLE_all <;> rfl
+
+@[simp]
+theorem Var?.add_idem_scopy {v : Var? α ε} (hv : v.scopy) : v + v = v := by
+  cases v with | mk A q e =>
+  simp only [add_def, mk.injEq, and_true, true_and]
+  cases hv.q using EQuant.le.casesLE_all <;> rfl
+
+theorem Var?.PSSplit.add_eq {u v w : Var? α ε} (h : u.PSSplit v w) : v + w = u := by
+  induction h <;> simp [*]
+
+theorem Ctx?.PSSplit.add_eq {Γ Δ Ξ : Ctx? α ε} (h : Γ.PSSplit Δ Ξ) : Δ + Ξ = Γ := by
+  induction h with | nil => rfl | cons hΓ hvw I => simp [I, hvw.add_eq]
